Differentiate source/target language, update pass to work on abs instead, and add some new tests

Definitions.v
@@ -27,245 +27,410 @@ these are terms that are introduced by the locally nameless style,
 but are invalid lc terms
 i.e. (bvar 1) with no context
 *)
-Inductive trm : Set :=
-  | trm_let (v : trm)(ts : list trm)
-  | trm_abs  (ts : list trm)
-  | trm_app  (t1 : trm)(t2 : trm)
-  | trm_set (x : trm)(t : trm)
-  | trm_setcar (pair : trm)(v : trm)
-  | trm_setcdr (pair : trm)(v : trm)
-  | trm_cons (v1 : trm)(v2 : trm)
-  | trm_car (pair : trm)
-  | trm_cdr (pair : trm)
-  | trm_bvar (i : nat)
-  | trm_fvar (x : var)
-  | trm_pp (n : var)
-  | trm_num (i : nat)
-  | trm_null
-  | trm_true
-  | trm_false
-  (*
-  | pre_begin (e : trm)(es : list trm)
-  | pre_begin0 (e : trm)(es : list trm)
-  *).
 
-Inductive value : trm -> Prop :=
-  | value_abs : forall ts,
-      value (trm_abs ts)
-  | value_pp : forall n,
-      value (trm_pp n)
-  | value_num : forall i,
-      value (trm_num i)
-  | value_null : value (trm_null)
-  | value_true : value (trm_true)
-  | value_false : value (trm_false).
+(*source langauge pre-terms*)
+Inductive s_trm : Set :=
+  | s_trm_abs  (ts : list s_trm)
+  | s_trm_app  (t1 : s_trm)(t2 : s_trm)
+  | s_trm_begin (ts : list s_trm)
+  | s_trm_set (x : s_trm)(t : s_trm)
+  | s_trm_setcar (pair : s_trm)(v : s_trm)
+  | s_trm_setcdr (pair : s_trm)(v : s_trm)
+  | s_trm_cons (v1 : s_trm)(v2 : s_trm)
+  | s_trm_car (pair : s_trm)
+  | s_trm_cdr (pair : s_trm)
+  | s_trm_bvar (i : nat)
+  | s_trm_fvar (x : var)
+  | s_trm_pp (n : var)
+  | s_trm_num (i : nat)
+  | s_trm_null
+  | s_trm_true
+  | s_trm_false.
+
+(* target language pre-terms*)
+Inductive t_trm : Set :=
+  | t_trm_abs  (ts : list t_trm)
+  | t_trm_app  (t1 : t_trm)(t2 : t_trm)
+  | t_trm_let (v : t_trm) (ts : list t_trm)
+  | t_trm_set_top (x : var) (t : t_trm)
+  | t_trm_begin (ts : list t_trm)
+  | t_trm_setcar (pair : t_trm)(v : t_trm)
+  | t_trm_setcdr (pair : t_trm)(v : t_trm)
+  | t_trm_cons (v1 : t_trm)(v2 : t_trm)
+  | t_trm_car (pair : t_trm)
+  | t_trm_cdr (pair : t_trm)
+  | t_trm_bvar (i : nat)
+  | t_trm_fvar (x : var)
+  | t_trm_pp (n : var)
+  | t_trm_num (i : nat)
+  | t_trm_null
+  | t_trm_true
+  | t_trm_false.
+
+Inductive s_val : s_trm -> Prop :=
+  | sval_abs : forall ts,
+      s_val (s_trm_abs ts)
+  | sval_pp : forall n,
+      s_val (s_trm_pp n)
+  | sval_num : forall i,
+      s_val (s_trm_num i)
+  | sval_null : s_val (s_trm_null)
+  | sval_true : s_val (s_trm_true)
+  | sval_false : s_val (s_trm_false).
+
+Inductive t_val : t_trm -> Prop :=
+  | tval_abs : forall ts,
+      t_val (t_trm_abs ts)
+  | tval_pp : forall n,
+      t_val (t_trm_pp n)
+  | tval_num : forall i,
+      t_val (t_trm_num i)
+  | tval_null : t_val (t_trm_null)
+  | tval_true : t_val (t_trm_true)
+  | tval_false : t_val (t_trm_false).
 
 (* 
 Opening a term t with a term u containing a fresh free variable x.
-  so u = (trm_var (fvar x))
+  so u = (s_trm_var (fvar x))
 To do so, we replace all references to local bvar with u.
 This means we have to keep track of the current level of abstraction with k
 So we are replacing all (bvar k) with (fvar x), and incrementing k with abstraction levels
 *)
 
-Fixpoint open_rec (k : nat) (u : trm) (t : trm) {struct t} : trm :=
+Fixpoint s_open_rec (k : nat) (u : s_trm) (t : s_trm) {struct t} : s_trm :=
   match t with
-  | trm_bvar i => if (k =? i) then u else t
-  | trm_fvar x => t
-  | trm_abs ts => let open_rec_S := (open_rec (S k) u) in
-                  trm_abs (map open_rec_S ts)
-  | trm_let b ts => let open_rec_S := (open_rec (S k) u) in
-                    trm_let (open_rec k u b) (map open_rec_S ts)
-  | trm_app t1 t2 => trm_app (open_rec k u t1)(open_rec k u t2)
-  | trm_set x t1 => trm_set (open_rec k u x) (open_rec k u t1)
-  | trm_setcar p v => trm_setcar (open_rec k u p) (open_rec k u v)
-  | trm_setcdr p v => trm_setcdr (open_rec k u p) (open_rec k u v)
-  | trm_cons v1 v2 => trm_cons (open_rec k u v1)(open_rec k u v2)
-  | trm_car p => trm_car (open_rec k u p)
-  | trm_cdr p => trm_cdr (open_rec k u p)
+  | s_trm_bvar i => if (k =? i) then u else t
+  | s_trm_fvar x => t
+  | s_trm_abs ts => let s_open_rec_S := (s_open_rec (S k) u) in
+                    s_trm_abs (map s_open_rec_S ts)
+  | s_trm_app t1 t2 => s_trm_app (s_open_rec k u t1)(s_open_rec k u t2)
+  | s_trm_set x t1 => s_trm_set (s_open_rec k u x) (s_open_rec k u t1)
+  | s_trm_setcar p v => s_trm_setcar (s_open_rec k u p) (s_open_rec k u v)
+  | s_trm_setcdr p v => s_trm_setcdr (s_open_rec k u p) (s_open_rec k u v)
+  | s_trm_cons v1 v2 => s_trm_cons (s_open_rec k u v1)(s_open_rec k u v2)
+  | s_trm_car p => s_trm_car (s_open_rec k u p)
+  | s_trm_cdr p => s_trm_cdr (s_open_rec k u p)
+  | s_trm_begin ts => let s_open_rec_S := (s_open_rec (S k) u) in
+                      s_trm_begin (map s_open_rec_S ts)
   | _ => t
   end.
 
-Notation "{ k ~> u } t" := (open_rec k u t) (at level 67).
+Fixpoint t_open_rec (k : nat) (u : t_trm) (t : t_trm) {struct t} : t_trm :=
+  match t with
+  | t_trm_bvar i => if (k =? i) then u else t
+  | t_trm_fvar x => t
+  | t_trm_abs ts => let t_open_rec_S := (t_open_rec (S k) u) in
+                    t_trm_abs (map t_open_rec_S ts)
+  | t_trm_let v ts => let t_open_rec_S := (t_open_rec (S k) u) in
+                      t_trm_let (t_open_rec k u v) (map t_open_rec_S ts)
+  | t_trm_set_top x t1 => t_trm_set_top x (t_open_rec k u t1)
+  | t_trm_app t1 t2 => t_trm_app (t_open_rec k u t1)(t_open_rec k u t2)
+  | t_trm_setcar p v => t_trm_setcar (t_open_rec k u p) (t_open_rec k u v)
+  | t_trm_setcdr p v => t_trm_setcdr (t_open_rec k u p) (t_open_rec k u v)
+  | t_trm_cons v1 v2 => t_trm_cons (t_open_rec k u v1)(t_open_rec k u v2)
+  | t_trm_car p => t_trm_car (t_open_rec k u p)
+  | t_trm_cdr p => t_trm_cdr (t_open_rec k u p)
+  | t_trm_begin ts => let t_open_rec_S := (t_open_rec (S k) u) in
+                      t_trm_begin (map t_open_rec_S ts)
+  | _ => t
+  end.
 
-Definition open t u := open_rec 0 u t.
+Notation "{ k ~>s u } t" := (s_open_rec k u t) (at level 67).
+Notation "{ k ~>t u } t" := (t_open_rec k u t) (at level 67).
 
-Notation "t ^^ u" := (open t u) (at level 67).
-Notation "t ^ x" := (open t (trm_fvar x)).
+Definition s_open t u := s_open_rec 0 u t.
+Definition t_open t u := t_open_rec 0 u t.
+
+Notation "t ^^s u" := (s_open t u) (at level 67).
+Notation "t ^s x" := (s_open t (s_trm_fvar x)) (at level 67).
+
+Notation "t ^^t u" := (t_open t u) (at level 67).
+Notation "t ^t x" := (t_open t (t_trm_fvar x)) (at level 67).
 
 (*
 Closing a term is the inverse of opening.
 Replaces a free var z with bvar n where n is the current level of abstraction
 *)
-Fixpoint close_var_rec (k : nat) (z : var) (t : trm) {struct t} : trm :=
+Fixpoint s_close_var_rec (k : nat) (z : var) (t : s_trm) {struct t} : s_trm :=
   match t with
-  | trm_bvar i => t
-  | trm_fvar x => if var_compare x z then (trm_bvar k) else t
-  | trm_abs ts => let close_var_rec_S := (close_var_rec (S k) z) in
-                  trm_abs (map close_var_rec_S ts)
-  | trm_let b ts => let close_var_rec_S := (close_var_rec (S k) z) in
-                    trm_let (close_var_rec k z b) (map close_var_rec_S ts)
-  | trm_app t1 t2 => trm_app (close_var_rec k z t1) (close_var_rec k z t2)
-  | trm_set x t1 => trm_set (close_var_rec k z x) (close_var_rec k z t1)
-  | trm_setcar p v => trm_setcar (close_var_rec k z p) (close_var_rec k z v)
-  | trm_setcdr p v => trm_setcdr (close_var_rec k z p) (close_var_rec k z v)
-  | trm_cons v1 v2 => trm_cons (close_var_rec k z v1) (close_var_rec k z v2)
-  | trm_car p => trm_car (close_var_rec k z p)
-  | trm_cdr p => trm_cdr (close_var_rec k z p)
+  | s_trm_bvar i => t
+  | s_trm_fvar x => if var_compare x z then (s_trm_bvar k) else t
+  | s_trm_abs ts => let s_close_var_rec_S := (s_close_var_rec (S k) z) in
+                  s_trm_abs (map s_close_var_rec_S ts)
+  | s_trm_app t1 t2 => s_trm_app (s_close_var_rec k z t1) (s_close_var_rec k z t2)
+  | s_trm_set x t1 => s_trm_set (s_close_var_rec k z x) (s_close_var_rec k z t1)
+  | s_trm_setcar p v => s_trm_setcar (s_close_var_rec k z p) (s_close_var_rec k z v)
+  | s_trm_setcdr p v => s_trm_setcdr (s_close_var_rec k z p) (s_close_var_rec k z v)
+  | s_trm_cons v1 v2 => s_trm_cons (s_close_var_rec k z v1) (s_close_var_rec k z v2)
+  | s_trm_car p => s_trm_car (s_close_var_rec k z p)
+  | s_trm_cdr p => s_trm_cdr (s_close_var_rec k z p)
+  | s_trm_begin ts => s_trm_begin (map (s_close_var_rec k z) ts)
   | _ => t
   end.
 
-Definition close_var z t := close_var_rec 0 z t.
-Fixpoint open_each ts x :=
-  match ts with
-  | [] => []
-  | t :: ts' => (t ^ x) :: open_each ts' x
+Fixpoint t_close_var_rec (k : nat) (z : var) (t : t_trm) {struct t} : t_trm :=
+  match t with
+  | t_trm_bvar i => t
+  | t_trm_fvar x => if var_compare x z then (t_trm_bvar k) else t
+  | t_trm_abs ts => let t_close_var_rec_S := (t_close_var_rec (S k) z) in
+                  t_trm_abs (map t_close_var_rec_S ts)
+  | t_trm_app t1 t2 => t_trm_app (t_close_var_rec k z t1) (t_close_var_rec k z t2)
+  | t_trm_setcar p v => t_trm_setcar (t_close_var_rec k z p) (t_close_var_rec k z v)
+  | t_trm_setcdr p v => t_trm_setcdr (t_close_var_rec k z p) (t_close_var_rec k z v)
+  | t_trm_cons v1 v2 => t_trm_cons (t_close_var_rec k z v1) (t_close_var_rec k z v2)
+  | t_trm_car p => t_trm_car (t_close_var_rec k z p)
+  | t_trm_cdr p => t_trm_cdr (t_close_var_rec k z p)
+  | t_trm_begin ts => t_trm_begin (map (t_close_var_rec k z) ts)
+  | _ => t
   end.
 
-Fixpoint open_each_term ts u :=
+Definition s_close_var z t := s_close_var_rec 0 z t.
+Definition t_close_var z t := t_close_var_rec 0 z t.
+
+Fixpoint s_open_each ts x :=
   match ts with
   | [] => []
-  | t :: ts' => (t ^^ u) :: open_each_term ts' u
+  | t :: ts' => (t ^s x) :: s_open_each ts' x
+  end.
+
+Fixpoint t_open_each ts x :=
+  match ts with
+  | [] => []
+  | t :: ts' => (t ^t x) :: t_open_each ts' x
+  end.
+
+Fixpoint s_open_each_term ts u :=
+  match ts with
+  | [] => []
+  | t :: ts' => (t ^^s u) :: s_open_each_term ts' u
   end.
   
+Fixpoint t_open_each_term ts u :=
+  match ts with
+  | [] => []
+  | t :: ts' => (t ^^s u) :: t_open_each_term ts' u
+  end.
 
+Inductive s_term : s_trm -> Prop :=
+  | s_term_fvar : forall x,
+      s_term (s_trm_fvar x)
+  | s_term_app : forall t1 t2,
+      s_term t1 -> s_term t2 -> s_term (s_trm_app t1 t2)
+  | s_term_abs : forall L ts,
+      (forall x, x \notin L -> s_terms (s_open_each ts x)) ->
+      s_term (s_trm_abs ts)
+  | s_term_begin : forall L ts,
+      (forall x, x \notin L -> s_terms (s_open_each ts x)) ->
+      s_term (s_trm_begin ts)
+  | s_term_set : forall b t,
+      s_term b -> s_term t -> s_term (s_trm_set b t)
+  | s_term_setcar : forall p v,
+      s_term p -> s_term v -> s_term (s_trm_setcar p v)
+  | s_term_setcdr : forall p v,
+      s_term p -> s_term v -> s_term (s_trm_setcdr p v)
+  | s_term_cons : forall v1 v2, 
+      s_term v1 -> s_term v2 -> s_term (s_trm_cons v1 v2)
+  | s_term_car : forall p,
+      s_term p -> s_term (s_trm_car p)
+  | s_term_cdr : forall p,
+      s_term p -> s_term (s_trm_cdr p)
+  | s_term_pp : forall n,
+      s_term (s_trm_pp n)
+  | s_term_num : forall i,
+      s_term (s_trm_num i)
+  | s_term_null : s_term (s_trm_null)
+  | s_term_true : s_term (s_trm_true)
+  | s_term_false : s_term (s_trm_false)
 
-Inductive term : trm -> Prop :=
-  | term_fvar : forall x,
-      term (trm_fvar x)
-  | term_app : forall t1 t2,
-      term t1 -> term t2 -> term (trm_app t1 t2)
-  | term_abs : forall L ts,
-      (forall x, x \notin L -> terms (open_each ts x)) ->
-      term (trm_abs ts)
-      (* (forall x, x \notin L -> term (t ^ x)) ->
-      term (trm_abs ts) *)
-  | term_let : forall L ts t b,
-      term b ->
-      In t ts ->
-      (forall x, x \notin L -> terms (open_each ts x)) ->
-      term (trm_let b ts)
-  | term_set : forall b t,
-      term b -> term t -> term (trm_set b t)
-  | term_setcar : forall p v,
-      term p -> term v -> term (trm_setcar p v)
-  | term_setcdr : forall p v,
-      term p -> term v -> term (trm_setcdr p v)
-  | term_cons : forall v1 v2, 
-      term v1 -> term v2 -> term (trm_cons v1 v2)
-  | term_car : forall p,
-      term p -> term (trm_car p)
-  | term_cdr : forall p,
-      term p -> term (trm_cdr p)
-  | term_pp : forall n,
-      term (trm_pp n)
-  | term_num : forall i,
-      term (trm_num i)
-  | term_null : term (trm_null)
-  | term_true : term (trm_true)
-  | term_false : term (trm_false)
-
-with terms : list trm -> Prop :=
-  | terms_nil : terms ([])
-  | terms_single : forall t, term t -> terms [t]
-  | terms_next : 
+with s_terms : list s_trm -> Prop :=
+  | s_terms_nil : s_terms ([])
+  | s_terms_single : forall t, s_term t -> s_terms [t]
+  | s_terms_next : 
       forall t ts,
-        terms ts -> 
-        term t ->
-        terms (t :: ts).
-                 
+        s_terms ts -> 
+        s_term t ->
+        s_terms (t :: ts).
 
+
+Inductive t_term : t_trm -> Prop :=
+  | t_term_fvar : forall x,
+      t_term (t_trm_fvar x)
+  | t_term_app : forall t1 t2,
+      t_term t1 -> t_term t2 -> t_term (t_trm_app t1 t2)
+  | t_term_abs : forall L ts,
+      (forall x, x \notin L -> t_terms (t_open_each ts x)) ->
+      t_term (t_trm_abs ts)
+  | t_term_begin : forall L ts,
+      (forall x, x \notin L -> t_terms (t_open_each ts x)) ->
+      t_term (t_trm_begin ts)
+  | t_term_let : forall L ts t b,
+      t_term b ->
+      In t ts ->
+      (forall x, x \notin L -> t_terms (t_open_each ts x)) ->
+      t_term (t_trm_let b ts)
+  | t_term_setcar : forall p v,
+      t_term p -> t_term v -> t_term (t_trm_setcar p v)
+  | t_term_setcdr : forall p v,
+      t_term p -> t_term v -> t_term (t_trm_setcdr p v)
+  | t_term_cons : forall v1 v2, 
+      t_term v1 -> t_term v2 -> t_term (t_trm_cons v1 v2)
+  | t_term_car : forall p,
+      t_term p -> t_term (t_trm_car p)
+  | t_term_cdr : forall p,
+      t_term p -> t_term (t_trm_cdr p)
+  | t_term_pp : forall n,
+      t_term (t_trm_pp n)
+  | t_term_num : forall i,
+      t_term (t_trm_num i)
+  | t_term_null : t_term (t_trm_null)
+  | t_term_true : t_term (t_trm_true)
+  | t_term_false : t_term (t_trm_false)
+
+with t_terms : list t_trm -> Prop :=
+  | t_terms_nil : t_terms ([])
+  | t_terms_single : forall t, t_term t -> t_terms [t]
+  | t_terms_next : 
+      forall t ts,
+        t_terms ts -> 
+        t_term t ->
+        t_terms (t :: ts).
 
 
 (* Body of an abstraction *)
-Definition body ts :=
+Definition s_body ts :=
   exists L,
-  forall x, x \notin L -> terms (open_each ts x).
+  forall x, x \notin L -> s_terms (s_open_each ts x).
 
-Fixpoint big_unionf (ts : list trm) (f : trm -> vars) : vars :=
-  match ts with
-  | [] => \{}
-  | t :: ts' => f t \u big_unionf ts' f
-  end.
+Definition t_body ts :=
+  exists L,
+  forall x, x \notin L -> t_terms (t_open_each ts x).
 
-(* Free variables of a term *)
-Fixpoint fv (t : trm) : vars :=
-  let fix fvs' (ts : list trm) : vars :=
+(* Free variables of a source term *)
+Fixpoint s_fv (t : s_trm) : vars :=
+  let fix fvs' (ts : list s_trm) : vars :=
     match ts with
     | [] => \{}
-    | t :: ts' => fv t \u fvs' ts'
+    | t :: ts' => s_fv t \u fvs' ts'
     end
   in
     match t with
-    | trm_fvar y => \{y}
-    | trm_bvar _ => \{}
-    | trm_let b ts => (fv b) \u (fvs' ts) (* @fold_left (vars) (vars) (@union var) (map fv (b :: ts)) \{} *)
-    | trm_abs ts => fvs' ts (* @fold_left (vars) (vars) (@union var) (map fv ts) \{} *)
-    | trm_app t1 t2 => (fv t1) \u (fv t2)
-    | trm_set x t1 => (fv x) \u (fv t1)
-    | trm_setcar p v => (fv p) \u (fv v)
-    | trm_setcdr p v => (fv p) \u (fv v)
-    | trm_cons v1 v2 => (fv v1) \u (fv v2)
-    | trm_car p => fv p
-    | trm_cdr p => fv p
+    | s_trm_fvar y => \{y}
+    | s_trm_bvar _ => \{}
+    | s_trm_abs ts => fvs' ts
+    | s_trm_begin ts => fvs' ts
+    | s_trm_app t1 t2 => (s_fv t1) \u (s_fv t2)
+    | s_trm_set x t1 => (s_fv x) \u (s_fv t1)
+    | s_trm_setcar p v => (s_fv p) \u (s_fv v)
+    | s_trm_setcdr p v => (s_fv p) \u (s_fv v)
+    | s_trm_cons v1 v2 => (s_fv v1) \u (s_fv v2)
+    | s_trm_car p => s_fv p
+    | s_trm_cdr p => s_fv p
     | _ => \{}
     end.
 
-Fixpoint fvs (ts : list trm) : vars :=
-  match ts with 
-  | [] => \{}
-  | t :: ts' => fv t \u fvs ts'
-  end.
+Fixpoint t_fv (t : t_trm) : vars :=
+  let fix fvs' (ts : list t_trm) : vars :=
+    match ts with
+    | [] => \{}
+    | t :: ts' => t_fv t \u fvs' ts'
+    end
+  in
+    match t with
+    | t_trm_fvar y => \{y}
+    | t_trm_bvar _ => \{}
+    | t_trm_abs ts => fvs' ts
+    | t_trm_begin ts => fvs' ts
+    | t_trm_app t1 t2 => (t_fv t1) \u (t_fv t2)
+    | t_trm_set_top x t1 => \{x} \u (t_fv t1)
+    | t_trm_setcar p v => (t_fv p) \u (t_fv v)
+    | t_trm_setcdr p v => (t_fv p) \u (t_fv v)
+    | t_trm_cons v1 v2 => (t_fv v1) \u (t_fv v2)
+    | t_trm_car p => t_fv p
+    | t_trm_cdr p => t_fv p
+    | _ => \{}
+    end.
 
-Fixpoint subst (z : var) (u : trm) (t : trm) {struct t} : trm :=
-  let fix substs (ts : list trm) :=
+Fixpoint s_subst (z : var) (u : s_trm) (t : s_trm) {struct t} : s_trm :=
+  let fix substs (ts : list s_trm) :=
     match ts with
     | [] => []
-    | t' :: ts' => (subst z u t') :: (substs ts')
+    | t' :: ts' => (s_subst z u t') :: (substs ts')
     end
   in
   match t with
-  | trm_let v ts => trm_let (subst z u v) (substs ts)
-  | trm_abs ts => trm_abs (substs ts)
-  | trm_app t1 t2 => trm_app (subst z u t1) (subst z u t2)
-  | trm_set x t1 => trm_set (subst z u x) (subst z u t1)
-  | trm_setcar p v => trm_setcar (subst z u p) (subst z u v)
-  | trm_setcdr p v => trm_setcdr (subst z u p) (subst z u v)
-  | trm_cons v1 v2 => trm_cons (subst z u v1) (subst z u v2)
-  | trm_car p => trm_car (subst z u p)
-  | trm_cdr p => trm_cdr (subst z u p)
-  | trm_fvar x => if (var_compare x z) then u else t
-  | trm_bvar i => t
+  | s_trm_abs ts => s_trm_abs (substs ts)
+  | s_trm_begin ts => s_trm_begin (substs ts)
+  | s_trm_app t1 t2 => s_trm_app (s_subst z u t1) (s_subst z u t2)
+  | s_trm_set x t1 => s_trm_set (s_subst z u x) (s_subst z u t1)
+  | s_trm_setcar p v => s_trm_setcar (s_subst z u p) (s_subst z u v)
+  | s_trm_setcdr p v => s_trm_setcdr (s_subst z u p) (s_subst z u v)
+  | s_trm_cons v1 v2 => s_trm_cons (s_subst z u v1) (s_subst z u v2)
+  | s_trm_car p => s_trm_car (s_subst z u p)
+  | s_trm_cdr p => s_trm_cdr (s_subst z u p)
+  | s_trm_fvar x => if (var_compare x z) then u else t
+  | s_trm_bvar i => t
   | _ => t
   end.
 
-Notation "[ z ~> u ] t" := (subst z u t) (at level 68).
+Fixpoint t_subst (z : var) (u : t_trm) (t : t_trm) {struct t} : t_trm :=
+  let fix substs (ts : list t_trm) :=
+    match ts with
+    | [] => []
+    | t' :: ts' => (t_subst z u t') :: (substs ts')
+    end
+  in
+  match t with
+  | t_trm_abs ts => t_trm_abs (substs ts)
+  | t_trm_begin ts => t_trm_begin (substs ts)
+  | t_trm_app t1 t2 => t_trm_app (t_subst z u t1) (t_subst z u t2)
+  | t_trm_let v ts => t_trm_let (t_subst z u v) (substs ts)
+  | t_trm_setcar p v => t_trm_setcar (t_subst z u p) (t_subst z u v)
+  | t_trm_setcdr p v => t_trm_setcdr (t_subst z u p) (t_subst z u v)
+  | t_trm_cons v1 v2 => t_trm_cons (t_subst z u v1) (t_subst z u v2)
+  | t_trm_car p => t_trm_car (t_subst z u p)
+  | t_trm_cdr p => t_trm_cdr (t_subst z u p)
+  | t_trm_fvar x => if (var_compare x z) then u else t
+  | t_trm_bvar i => t
+  | _ => t
+  end.
 
-(* Definition sum (A : Type) (l : list A) (f : A -> nat) :=
-  (fold_left
-   (fun a x => a + x)
-   0
-   (map f l)).
-*)
+Notation "[ z ~>s u ] t" := (s_subst z u t) (at level 68).
+Notation "[ z ~>t u ] t" := (t_subst z u t) (at level 68).
 
 Definition sum (l : list nat) :=
   fold_left (plus) l 0.
 
-Fixpoint trm_size (t : trm) {struct t} : nat :=
+Fixpoint s_trm_size (t : s_trm) {struct t} : nat :=
   match t with
-  | trm_let v ts => 1 + (trm_size v) + (sum (map trm_size ts))
-  | trm_abs ts => 1 + (sum (map trm_size ts))
-  | trm_app t1 t2 => 1 + (trm_size t1) + (trm_size t2)
-  | trm_set x t1 => 1 + (trm_size x) + (trm_size t1)
-  | trm_setcar p v => 1 + (trm_size p) + (trm_size v)
-  | trm_setcdr p v => 1 + (trm_size p) + (trm_size v)
-  | trm_cons v1 v2 => 1 + (trm_size v1) + (trm_size v2)
-  | trm_car p => 1 + (trm_size p)
-  | trm_cdr p => 1 + (trm_size p)
-  | trm_fvar _ => 1
-  | trm_bvar _ => 1
+  | s_trm_abs ts => 1 + (sum (map s_trm_size ts))
+  | s_trm_begin ts => 1 + (sum (map s_trm_size ts))
+  | s_trm_app t1 t2 => 1 + (s_trm_size t1) + (s_trm_size t2)
+  | s_trm_set x t1 => 1 + (s_trm_size x) + (s_trm_size t1)
+  | s_trm_setcar p v => 1 + (s_trm_size p) + (s_trm_size v)
+  | s_trm_setcdr p v => 1 + (s_trm_size p) + (s_trm_size v)
+  | s_trm_cons v1 v2 => 1 + (s_trm_size v1) + (s_trm_size v2)
+  | s_trm_car p => 1 + (s_trm_size p)
+  | s_trm_cdr p => 1 + (s_trm_size p)
+  | s_trm_fvar _ => 1
+  | s_trm_bvar _ => 1
   | _ => 1
   end.
 
+Fixpoint t_trm_size (t : t_trm) {struct t} : nat :=
+  match t with 
+  | t_trm_abs ts => 1 + (sum (map t_trm_size ts))
+  | t_trm_begin ts => 1 + (sum (map t_trm_size ts))
+  | t_trm_app t1 t2 => 1 + (t_trm_size t1) + (t_trm_size t2)
+  | t_trm_set_top x t1 => 2 + (t_trm_size t1)
+  | t_trm_let v ts => 1 + (t_trm_size v) + (sum (map t_trm_size ts))
+  | t_trm_setcar p v => 1 + (t_trm_size p) + (t_trm_size v)
+  | t_trm_setcdr p v => 1 + (t_trm_size p) + (t_trm_size v)
+  | t_trm_cons v1 v2 => 1 + (t_trm_size v1) + (t_trm_size v2)
+  | t_trm_car p => 1 + (t_trm_size p)
+  | t_trm_cdr p => 1 + (t_trm_size p)
+  | t_trm_fvar _ => 1
+  | t_trm_bvar _ => 1
+  | _ => 1
+  end.
 
 
