Examples.v
@@ -3,38 +3,30 @@ From vchez Require Export Pass.
 From Coq Require Import List.
 Import ListNotations.
 
+(* Examples of the convert-assignments pass working as intended *)
+
 Example ca_1 : forall x,
-  ca (trm_fvar x) = SomeE (trm_fvar x).
+  ca (s_trm_fvar x) = SomeE (t_trm_fvar x).
 Proof. reflexivity. Qed.
 
-Example ca_2 : forall v1 v2,
-  ca (trm_let v1 [trm_let v2 [trm_bvar 0]]) =
-  SomeE (trm_let v1 [trm_let v2 [trm_bvar 0]]).
+Example ca_2 :
+  ca (s_trm_abs [s_trm_set (s_trm_bvar 0) s_trm_true]) =
+  SomeE (t_trm_abs
+          [t_trm_let (t_trm_cons (t_trm_bvar 0) (t_trm_null))
+            [t_trm_setcar (t_trm_bvar 0) t_trm_true]]).
 Proof. reflexivity. Qed.
 
-Example ca_3 : forall v1 v2,
-  ca (trm_let v1 [trm_let v2 [trm_bvar 0; trm_bvar 1]]) =
-  SomeE (trm_let v1 [trm_let v2 [trm_bvar 0; trm_bvar 1]]).
+Example ca_6 :
+  ca (s_trm_app 
+       (s_trm_abs 
+         [s_trm_set (s_trm_bvar 0) s_trm_true;
+          s_trm_bvar 0])
+        s_trm_false) =
+  SomeE (t_trm_app 
+          (t_trm_abs
+            [t_trm_let (t_trm_cons (t_trm_bvar 0) (t_trm_null))
+              [t_trm_setcar (t_trm_bvar 0) t_trm_true;
+               t_trm_car (t_trm_bvar 0)]])
+          t_trm_false).
 Proof. reflexivity. Qed.
-
-Example ca_4 : forall v1,
-  ca (trm_let v1 [trm_bvar 0]) =
-  SomeE (trm_let v1 [trm_bvar 0]).
-Proof. reflexivity. Qed.
-
-Example ca_5 :
-  ca (trm_let trm_false
-       [trm_set (trm_bvar 0) trm_true]) =
-  SomeE (trm_let trm_false
-          [trm_let (trm_cons (trm_bvar 0) (trm_null)) 
-            [trm_setcar (trm_bvar 0) trm_true]]).
-Proof. reflexivity. Qed.
-
-
-(*These examples show the algorithm for finding set! that refer to a variable bound by a let*)
-Example set1 :
-  handle_sets (trm_set (trm_bvar 0) (trm_null)) =
-              SomeE (trm_setcar (trm_bvar 0) trm_null).
-Proof.
-  reflexivity. Qed.
 
