Pass.v
@@ -29,28 +29,27 @@ Notation "' p <- e1 ;; e2"
 Definition orb_e t1 t2 :=
   ' c1 <- t1 ;; ' c2 <- t2 ;; SomeE (orb c1 c2).
 
-Fixpoint has_assigning_set (n i : nat) (t : trm) :=
+Fixpoint has_assigning_set (n i : nat) (t : s_trm) :=
   match n with 
   | O => NoneE "Too many recursive calls"
   | S n' => 
     match t with
-    | trm_let v ts => has_assigning_set_list n' (S i) ts
-    | trm_abs ts => has_assigning_set_list n' (S i) ts
-    | trm_app t1 t2 => orb_e (has_assigning_set n' i t1) (has_assigning_set n' i t2)
-    | trm_set x t1 => match x with
-                      | (trm_bvar n) => if (i =? n) then SomeE true else has_assigning_set n' i t1
+    | s_trm_abs ts => has_assigning_set_list n' (S i) ts
+    | s_trm_app t1 t2 => orb_e (has_assigning_set n' i t1) (has_assigning_set n' i t2)
+    | s_trm_set x t1 => match x with
+                      | (s_trm_bvar n) => if (i =? n) then SomeE true else has_assigning_set n' i t1
                       | _ => has_assigning_set n' i t1
                       end
-    | trm_setcar p v => orb_e (has_assigning_set n' i p) (has_assigning_set n' i v)
-    | trm_setcdr p v => orb_e (has_assigning_set n' i p) (has_assigning_set n' i v)
-    | trm_cons v1 v2 => orb_e (has_assigning_set n' i v1) (has_assigning_set n' i v2)
-    | trm_car p => (has_assigning_set n' i p)
-    | trm_cdr p => (has_assigning_set n' i p)
+    | s_trm_setcar p v => orb_e (has_assigning_set n' i p) (has_assigning_set n' i v)
+    | s_trm_setcdr p v => orb_e (has_assigning_set n' i p) (has_assigning_set n' i v)
+    | s_trm_cons v1 v2 => orb_e (has_assigning_set n' i v1) (has_assigning_set n' i v2)
+    | s_trm_car p => (has_assigning_set n' i p)
+    | s_trm_cdr p => (has_assigning_set n' i p)
     | _ => SomeE false
     end
   end
 
-with has_assigning_set_list (n i : nat) (ts : list trm) :=
+with has_assigning_set_list (n i : nat) (ts : list s_trm) :=
   match n with 
   | O => NoneE "Too many recursive calls"
   | S n' => 
@@ -60,40 +59,40 @@ with has_assigning_set_list (n i : nat) (ts : list trm) :=
     end
   end.
 
-Fixpoint handle_assigning_set (n i : nat) (t : trm) :=
+Fixpoint handle_assigning_set (n i : nat) (t : s_trm) :=
   match n with 
   | O => NoneE "Too many recursive calls"
   | S n' =>
     match t with
-    | trm_let v ts =>   ' ts' <- (handle_assigning_set_list n' (S i) ts) ;; SomeE (trm_let v ts')
-    | trm_abs ts =>     ' ts' <- (handle_assigning_set_list n' (S i) ts) ;; SomeE (trm_abs ts')
-    | trm_bvar n =>     if (i =? n) then SomeE (trm_car (trm_bvar n)) else SomeE (trm_bvar n)
-    | trm_set x t1 =>   ' t1' <- (handle_assigning_set n' i t1) ;;
+    | s_trm_abs ts =>     ' ts' <- (handle_assigning_set_list n' (S i) ts) ;; 
+                          SomeE (s_trm_abs ts')
+    | s_trm_bvar n =>     if (i =? n) then SomeE (s_trm_car (s_trm_bvar n)) else SomeE (s_trm_bvar n)
+    | s_trm_set x t1 =>   ' t1' <- (handle_assigning_set n' i t1) ;;
                         match x with
-                        | trm_bvar n => if (i =? n) then SomeE (trm_setcar x t1') else SomeE (trm_set x t1')
-                        | _ => SomeE (trm_set x t1')
+                        | s_trm_bvar n => if (i =? n) then SomeE (s_trm_setcar x t1') else SomeE (s_trm_set x t1')
+                        | _ => SomeE (s_trm_set x t1')
                         end
-    | trm_app t1 t2 =>  ' t1' <- (handle_assigning_set n' i t1) ;;
+    | s_trm_app t1 t2 =>  ' t1' <- (handle_assigning_set n' i t1) ;;
                         ' t2' <- (handle_assigning_set n' i t2) ;;
-                        SomeE (trm_app t1' t2')
-    | trm_setcar p v => ' p' <- (handle_assigning_set n' i p) ;;
+                        SomeE (s_trm_app t1' t2')
+    | s_trm_setcar p v => ' p' <- (handle_assigning_set n' i p) ;;
                         ' v' <- (handle_assigning_set n' i v) ;;
-                        SomeE (trm_setcar p' v')
-    | trm_setcdr p v => ' p' <- (handle_assigning_set n' i p) ;;
+                        SomeE (s_trm_setcar p' v')
+    | s_trm_setcdr p v => ' p' <- (handle_assigning_set n' i p) ;;
                         ' v' <- (handle_assigning_set n' i v) ;;
-                        SomeE (trm_setcdr p' v')
-    | trm_cons v1 v2 => ' v1' <- (handle_assigning_set n' i v1) ;;
+                        SomeE (s_trm_setcdr p' v')
+    | s_trm_cons v1 v2 => ' v1' <- (handle_assigning_set n' i v1) ;;
                         ' v2' <- (handle_assigning_set n' i v2) ;;
-                        SomeE (trm_cons v1' v2')
-    | trm_car p =>      ' p' <- (handle_assigning_set n' i p) ;;
-                        SomeE (trm_car p')
-    | trm_cdr p =>      ' p' <- (handle_assigning_set n' i p) ;;
-                        SomeE (trm_cdr p')
+                        SomeE (s_trm_cons v1' v2')
+    | s_trm_car p =>      ' p' <- (handle_assigning_set n' i p) ;;
+                        SomeE (s_trm_car p')
+    | s_trm_cdr p =>      ' p' <- (handle_assigning_set n' i p) ;;
+                        SomeE (s_trm_cdr p')
     | t => SomeE t
     end
   end
 
-with handle_assigning_set_list (n i : nat) (ts : list trm) :=
+with handle_assigning_set_list (n i : nat) (ts : list s_trm) :=
   match n with
   | O => NoneE "Too many recursive calls"
   | S n' =>
@@ -111,45 +110,54 @@ Definition handle_sets_list := handle_assigning_set_list big_num 0.
 Definition has_sets := has_assigning_set big_num 0.
 Definition has_sets_list := has_assigning_set_list big_num 0.
 
-Fixpoint convert_assignments (n : nat) (t : trm) :=
+Fixpoint convert_assignments (n : nat) (t : s_trm) : OptionE t_trm :=
   match n with
   | O => NoneE "Too many recursive calls"
   | S n' =>
     match t with
-    | trm_let v ts => ' ts_has_set <- (has_sets_list ts) ;;
+    | s_trm_abs ts => ' ts_has_set <- (has_sets_list ts) ;;
                       if ts_has_set then
-                        ' body <- (handle_sets_list ts) ;;
-                        ' body' <- (convert_assignments_list n' body) ;;
-                        SomeE (trm_let v
-                                [trm_let (trm_cons (trm_bvar 0) (trm_null)) body'])
+                        ' body <- handle_sets_list ts ;;
+                        ' body' <- convert_assignments_list n' body ;;
+                        SomeE (t_trm_abs 
+                                [t_trm_let (t_trm_cons (t_trm_bvar 0) (t_trm_null))
+                                  body'])
                       else
-                        ' body <- (convert_assignments_list n' ts) ;;
-                        SomeE (trm_let v body)
-    | trm_fvar x => SomeE (trm_fvar x)
-    | trm_abs ts => ' body <- (convert_assignments_list n' ts) ;;
-                    SomeE (trm_abs body)
-    | trm_app t1 t2 => ' t1' <- (convert_assignments n' t1) ;;
-                       ' t2' <- (convert_assignments n' t2) ;;
-                       SomeE (trm_app t1' t2')
-    | trm_set x t1 => ' t1' <- (convert_assignments n' t1) ;;
-                      SomeE (trm_set x t1')
-    | trm_setcar p v => ' p' <- (convert_assignments n' p) ;;
-                        ' v' <- (convert_assignments n' v) ;;
-                        SomeE (trm_setcar p' v')
-    | trm_setcdr p v => ' p' <- (convert_assignments n' p) ;;
-                        ' v' <- (convert_assignments n' v) ;;
-                        SomeE (trm_setcdr p' v')
-    | trm_cons v1 v2 => ' v1' <- (convert_assignments n' v1) ;;
-                        ' v2' <- (convert_assignments n' v2) ;;
-                        SomeE (trm_cons v1' v2')
-    | trm_car p =>      ' p' <- (convert_assignments n' p) ;;
-                        SomeE (trm_car p')
-    | trm_cdr p =>      ' p' <- (convert_assignments n' p) ;;
-                        SomeE (trm_cdr p')
-    | t' => SomeE t'
+                        ' body <- convert_assignments_list n' ts ;;
+                        SomeE (t_trm_abs body)
+    | s_trm_app t1 t2 => ' t1' <- (convert_assignments n' t1) ;;
+                         ' t2' <- (convert_assignments n' t2) ;;
+                         SomeE (t_trm_app t1' t2')
+    | s_trm_begin ts =>  ' ts' <- (convert_assignments_list n' ts) ;;
+                         SomeE (t_trm_begin ts')
+    | s_trm_set x t1 => ' t1' <- (convert_assignments n' t1) ;;
+                          match x with 
+                          | s_trm_fvar y => SomeE (t_trm_set_top y t1')
+                          | _ => NoneE "Set applied to invalid bound variable"
+                          end
+    | s_trm_setcar p v => ' p' <- (convert_assignments n' p) ;;
+                          ' v' <- (convert_assignments n' v) ;;
+                          SomeE (t_trm_setcar p' v')
+    | s_trm_setcdr p v => ' p' <- (convert_assignments n' p) ;;
+                          ' v' <- (convert_assignments n' v) ;;
+                          SomeE (t_trm_setcdr p' v')
+    | s_trm_cons v1 v2 => ' v1' <- (convert_assignments n' v1) ;;
+                          ' v2' <- (convert_assignments n' v2) ;;
+                          SomeE (t_trm_cons v1' v2')
+    | s_trm_car p =>      ' p' <- (convert_assignments n' p) ;;
+                          SomeE (t_trm_car p')
+    | s_trm_cdr p =>      ' p' <- (convert_assignments n' p) ;;
+                          SomeE (t_trm_cdr p')
+    | s_trm_bvar i => SomeE (t_trm_bvar i)
+    | s_trm_fvar x => SomeE (t_trm_fvar x)
+    | s_trm_pp i => SomeE (t_trm_pp i)
+    | s_trm_num i => SomeE (t_trm_num i)
+    | s_trm_null => SomeE t_trm_null
+    | s_trm_true => SomeE t_trm_true
+    | s_trm_false => SomeE t_trm_false
     end
   end
-with convert_assignments_list (n : nat) (ts : list trm) :=
+with convert_assignments_list (n : nat) (ts : list s_trm) :=
   match n with
   | O => NoneE "Too many recursive calls"
   | S n' =>
@@ -160,6 +168,18 @@ with convert_assignments_list (n : nat) (ts : list trm) :=
                   SomeE (e_t :: e_ts)
     end
   end.
+
+
+(*    | s_trm_let v ts => ' ts_has_set <- (has_sets_list ts) ;;
+                      if ts_has_set then
+                        ' body <- (handle_sets_list ts) ;;
+                        ' body' <- (convert_assignments_list n' body) ;;
+                        SomeE (s_trm_let v
+                                [s_trm_let (s_trm_cons (s_trm_bvar 0) (s_trm_null)) body'])
+                      else
+                        ' body <- (convert_assignments_list n' ts) ;;
+                        SomeE (s_trm_let v body)
+*)
 
 Definition ca t :=
   convert_assignments big_num t.
